@prefix : <https://w3id.org/sulo/> .
@prefix owl: <http://www.w3.org/2002/07/owl#> .
@prefix rdf: <http://www.w3.org/1999/02/22-rdf-syntax-ns#> .
@prefix xml: <http://www.w3.org/XML/1998/namespace> .
@prefix xsd: <http://www.w3.org/2001/XMLSchema#> .
@prefix rdfs: <http://www.w3.org/2000/01/rdf-schema#> .
@base <https://w3id.org/sulo/> .

<https://w3id.org/sulo> rdf:type owl:Ontology ;
                         rdfs:comment "The Simplified Upper Level Ontology (SULO) is ontology with a minimal set of classes and relations to guide the development of a personal health knowledge graph."@en ;
                         rdfs:label "Simplified Upper Level Ontology"@en .

#################################################################
#    Object Properties
#################################################################

###  https://w3id.org/sulo/describes
:describes rdf:type owl:ObjectProperty ;
           rdfs:subPropertyOf :refersTo ;
           rdfs:comment "describes is a relation between an information object and the thing it provides a description for."@en ;
           rdfs:label "describes"@en .


###  https://w3id.org/sulo/encodes
:encodes rdf:type owl:ObjectProperty ;
         rdfs:subPropertyOf :refersTo ;
         rdfs:comment "A relation between an information containing object, in which the first object contains information that is used to produce the second object."@en ;
         rdfs:label "encodes"@en .


###  https://w3id.org/sulo/hasAttribute
:hasAttribute rdf:type owl:ObjectProperty ;
              rdfs:domain owl:Thing ;
              rdfs:range [ rdf:type owl:Class ;
                           owl:unionOf ( :Attribute
                                         :InformationObject
                                       )
                         ] ;
              rdfs:label "has attribute"@en .


###  https://w3id.org/sulo/hasDirectPart
:hasDirectPart rdf:type owl:ObjectProperty ;
               rdfs:subPropertyOf :hasPart ;
               rdfs:comment "has direct part is a parthood relation that can be used to specify cardinality constraints" ;
               rdfs:label "has direct part" .


###  https://w3id.org/sulo/hasPart
:hasPart rdf:type owl:ObjectProperty ;
         rdfs:subPropertyOf :isLocationOf ;
         owl:propertyDisjointWith :hasParticipant ;
         rdfs:label "has part"@en .


###  https://w3id.org/sulo/hasParticipant
:hasParticipant rdf:type owl:ObjectProperty ;
                rdfs:domain :Process ;
                rdfs:range [ rdf:type owl:Class ;
                             owl:unionOf ( :Attribute
                                           :InformationObject
                                           :SpatialObject
                                         )
                           ] ;
                rdfs:label "has participant"@en .


###  https://w3id.org/sulo/isLocationOf
:isLocationOf rdf:type owl:ObjectProperty ,
                       owl:TransitiveProperty ;
              rdfs:label "is location of"@en .


###  https://w3id.org/sulo/occursIn
:occursIn rdf:type owl:ObjectProperty ;
          rdfs:subPropertyOf owl:topObjectProperty ;
          rdfs:domain owl:Thing ;
          rdfs:range :Time ;
          rdfs:label "occurs in"@en .


###  https://w3id.org/sulo/refersTo
:refersTo rdf:type owl:ObjectProperty ;
          rdfs:label "refers to"@en .


###  https://w3id.org/sulo/represents
:represents rdf:type owl:ObjectProperty ;
            rdfs:subPropertyOf :refersTo ;
            rdfs:comment "a represents b when a serves as a sign, symbol or model of b."@en ;
            rdfs:label "represents"@en .


#################################################################
#    Data properties
#################################################################

###  https://w3id.org/sulo/hasValue
:hasValue rdf:type owl:DatatypeProperty ;
          rdfs:domain :InformationObject ;
          rdfs:comment "has value is the (only) data type attribute to store the values of information objects."@en ;
          rdfs:label "has value"@en .


#################################################################
#    Classes
#################################################################

###  https://w3id.org/sulo/ActionSpecification
:ActionSpecification rdf:type owl:Class ;
                     rdfs:subClassOf :InformationObject ;
                     rdfs:comment "An action specification is an information object composed of a sequence of instructions to achieve some objective"@en ;
                     rdfs:label "action specification"@en .


###  https://w3id.org/sulo/Attribute
:Attribute rdf:type owl:Class ;
           rdfs:subClassOf [ rdf:type owl:Restriction ;
                             owl:onProperty [ owl:inverseOf :hasAttribute
                                            ] ;
                             owl:someValuesFrom [ rdf:type owl:Class ;
                                                  owl:unionOf ( :Object
                                                                :Process
                                                              )
                                                ]
                           ] ;
           owl:disjointUnionOf ( :Capability
                                 :Quality
                                 :Role
                               ) ;
           rdfs:comment "An attribute is a property of an object or process that stems from their intrisinc structure and/or contextual interactions."@en ;
           rdfs:label "attribute"@en .


###  https://w3id.org/sulo/Capability
:Capability rdf:type owl:Class ;
            rdfs:subClassOf :Attribute ;
            rdfs:comment "A capability is an attribute that describes what an entity is able to do, under some set of circumstances."@en ,
                         "the capability to fly, the capabilty to reduce the activation energy of a chemical reaction, the capability to reason"@en ;
            rdfs:label "capability" .


###  https://w3id.org/sulo/Duration
:Duration rdf:type owl:Class ;
          rdfs:subClassOf :TimeInterval .


###  https://w3id.org/sulo/EndTime
:EndTime rdf:type owl:Class ;
         rdfs:subClassOf :TimeInstant ;
         rdfs:label "end time"@en .


###  https://w3id.org/sulo/InformationObject
:InformationObject rdf:type owl:Class ;
                   rdfs:subClassOf :Object ;
                   owl:disjointWith :SpatialObject ;
                   rdfs:comment "an information object is an object that represents or encodes information. Information objects can be stored, transmitted, or processed to enable communication, reasoning, or decision-making."@en ;
                   rdfs:label "information object"@en .


###  https://w3id.org/sulo/Object
:Object rdf:type owl:Class ;
        rdfs:subClassOf [ rdf:type owl:Class ;
                          owl:complementOf [ rdf:type owl:Restriction ;
                                             owl:onProperty :hasPart ;
                                             owl:someValuesFrom :Process
                                           ]
                        ] ,
                        [ rdf:type owl:Restriction ;
                          owl:onProperty :hasPart ;
                          owl:allValuesFrom :Object
                        ] ;
        owl:disjointWith :Process ;
        rdfs:comment "An object is an entity that maintains its identity through time, and does not have temporal parts." ;
        rdfs:label "object"@en .


###  https://w3id.org/sulo/Process
:Process rdf:type owl:Class ;
         rdfs:subClassOf [ rdf:type owl:Restriction ;
                           owl:onProperty :hasPart ;
                           owl:allValuesFrom :Process
                         ] ;
         rdfs:comment "a process is a entity that unfolds in time and has temporal parts."@en ;
         rdfs:label "process"@en .


###  https://w3id.org/sulo/Quality
:Quality rdf:type owl:Class ;
         rdfs:subClassOf :Attribute ;
         owl:disjointWith :Role ;
         rdfs:comment "A quality is an attribute that is intrinsically associated with its bearer (or its parts)."@en ,
                      "the color of an apple, the smoothness of skin, the brightness of a star, the speed of an event"@en ;
         rdfs:label "quality"@en .


###  https://w3id.org/sulo/Quantity
:Quantity rdf:type owl:Class ;
          rdfs:subClassOf :InformationObject ;
          rdfs:comment "A quantity is an informational object that contains the magnitude (and unit) of an attribute."@en ;
          rdfs:label "quantity"@en .


###  https://w3id.org/sulo/Role
:Role rdf:type owl:Class ;
      rdfs:subClassOf :Attribute ;
      rdfs:comment "A role is an attribute that describes a context-dependent behaviour."@en ,
                   "a teacher, a student, a catalyst, a substrate, a product"@en ;
      rdfs:label "role"@en .


###  https://w3id.org/sulo/SpatialObject
:SpatialObject rdf:type owl:Class ;
               rdfs:subClassOf :Object ;
               rdfs:comment "A spatial object is an object that occupies space"@en ,
                            "a mountain, a planet, a photon, the lining of the stomach, the cavity of the stomach, the space between mars and earth"@en ;
               rdfs:label "spatial object"@en .


###  https://w3id.org/sulo/StartTime
:StartTime rdf:type owl:Class ;
           rdfs:subClassOf :TimeInstant ;
           rdfs:label "start time"@en .


###  https://w3id.org/sulo/Time
:Time rdf:type owl:Class ;
      rdfs:subClassOf :Quantity ,
                      [ rdf:type owl:Restriction ;
                        owl:onProperty :hasPart ;
                        owl:someValuesFrom :Unit
                      ] ;
      rdfs:comment "time is a quantity pertaining to the duration of some interval of time or a particular instant of time (against some frame of reference)."@en ;
      rdfs:label "time"@en .


###  https://w3id.org/sulo/TimeInstant
:TimeInstant rdf:type owl:Class ;
             rdfs:subClassOf :Time ;
             rdfs:label "time instant"@en .


###  https://w3id.org/sulo/TimeInterval
:TimeInterval rdf:type owl:Class ;
              rdfs:subClassOf :Time ;
              rdfs:label "time interval" .


###  https://w3id.org/sulo/Unit
:Unit rdf:type owl:Class ;
      rdfs:subClassOf :Quantity .


###  https://w3id.org/sulo/set
:set rdf:type owl:Class ;
     rdfs:subClassOf :InformationObject ;
     rdfs:comment "A set is a collection of things, for which there may be zero members."@en ;
     rdfs:label "set"@en .


###  Generated by the OWL API (version 4.5.26.2023-07-17T20:34:13Z) https://github.com/owlcs/owlapi
