@prefix : <https://w3id.org/sulo/> .
@prefix owl: <http://www.w3.org/2002/07/owl#> .
@prefix rdf: <http://www.w3.org/1999/02/22-rdf-syntax-ns#> .
@prefix xml: <http://www.w3.org/XML/1998/namespace> .
@prefix xsd: <http://www.w3.org/2001/XMLSchema#> .
@prefix rdfs: <http://www.w3.org/2000/01/rdf-schema#> .
@prefix mod: <https://w3id.org/mod#> .
@prefix dcterms: <http://purl.org/dc/terms/> .
@prefix cc: <http://creativecommons.org/ns#> .
@prefix omv: <http://omv.ontoware.org/2005/05/ontology#> .
@prefix foaf: <http://xmlns.com/foaf/0.1/> .
@prefix schema: <https://schema.org/> .
@prefix dcat: <http://www.w3.org/ns/dcat#> .
@prefix sulo: <https://w3id.org/sulo/> .

@base <https://w3id.org/sulo/> .

<https://w3id.org/sulo> rdf:type owl:Ontology ;
                         rdfs:comment "The Simplified Upper Level Ontology (SULO) is ontology with a minimal set of classes and relations to guide the development of a personal health knowledge graph."@en;
                         owl:versionInfo "0.1.0";
                         mod:hasRepresentationLanguage  omv:OWL ;
                         mod:hasSyntax <http://www.w3.org/ns/formats/Turtle> ;
                         dcterms:language <http://lexvo.org/id/iso639-1/en> ;
                         dcterms:license <https://creativecommons.org/publicdomain/zero/1.0>;
                         foaf:homepage <https://w3id.org/sulo/>;
                         dcterms:alternative "SULO"@en ;
                         dcterms:created "2024-11-11" ;
                         schema:funding "This work is partially supported by the AIDAVA project (GA 101057062), as part of the European Union's Horizon Europe research and innovation programme."@en ;
                         mod:prefLabelProperty           rdfs:label ;
                         mod:definitionProperty          rdfs:comment ;
                          dcat:accessURL                  <https://github.com/AIDAVA-DEV/sulo/blob/main/sulo.ttl> ;
                         rdfs:label "Simplified Upper Level Ontology"@en .

#################################################################
#    Annotation properties
#################################################################

###  http://www.w3.org/2004/02/skos/core#example
<http://www.w3.org/2004/02/skos/core#example> rdf:type owl:AnnotationProperty .


#################################################################
#    Object Properties
#################################################################

###  https://w3id.org/sulo/causes
sulo:causes rdf:type owl:ObjectProperty ;
            rdfs:subPropertyOf sulo:precedes ;
            rdfs:domain sulo:Process ;
            rdfs:range sulo:Process ;
            rdfs:comment "a relation between two processes a,b, where a precedes b, and a is a necessary condition for b to occur."@en ;
            rdfs:label "causes"@en .


###  https://w3id.org/sulo/describes
sulo:describes rdf:type owl:ObjectProperty ;
               rdfs:subPropertyOf sulo:refersTo ;
               rdfs:domain sulo:InformationObject ;
               rdfs:comment "describes is a relation between an information object and the thing it provides a description for."@en ;
               rdfs:label "describes"@en .


###  https://w3id.org/sulo/encodes
sulo:encodes rdf:type owl:ObjectProperty ;
             rdfs:subPropertyOf sulo:refersTo ;
             rdfs:comment "A relation between an information containing object, in which the first object contains information that is used to produce the second object."@en ;
             rdfs:label "encodes"@en .


###  https://w3id.org/sulo/hasAttribute
sulo:hasAttribute rdf:type owl:ObjectProperty ;
                  rdfs:domain owl:Thing ;
                  rdfs:range [ rdf:type owl:Class ;
                               owl:unionOf ( sulo:Attribute
                                             sulo:InformationObject
                                           )
                             ] ;
                  rdfs:comment "has attribute is a relation between a thing and an internal, contextual, or externally attributed characteristic."@en ;
                  rdfs:label "has attribute"@en .


###  https://w3id.org/sulo/hasDirectPart
sulo:hasDirectPart rdf:type owl:ObjectProperty ;
                   rdfs:subPropertyOf sulo:hasPart ;
                   rdfs:comment "has direct part is a non-transitive parthood relation that can be used to specify cardinality constraints."@en ;
                   rdfs:label "has direct part" .


###  https://w3id.org/sulo/hasMember
sulo:hasMember rdf:type owl:ObjectProperty ;
               rdfs:domain sulo:Set ;
               rdfs:comment "has item is a relation between a set and items in that set."@en ;
               rdfs:label "has item"@en .


###  https://w3id.org/sulo/hasPart
sulo:hasPart rdf:type owl:ObjectProperty ;
             rdfs:subPropertyOf sulo:isLocationOf ;
             rdf:type owl:TransitiveProperty ,
                      owl:ReflexiveProperty ;
             rdfs:comment "has part is a transitive, reflexive and antisymmetric relation between a whole and itself or a whole and its part." ;
             rdfs:label "has part"@en .


###  https://w3id.org/sulo/hasParticipant
sulo:hasParticipant rdf:type owl:ObjectProperty ;
                    rdfs:domain sulo:Process ;
                    rdfs:range [ rdf:type owl:Class ;
                                 owl:unionOf ( sulo:Attribute
                                               sulo:Object
                                             )
                               ] ,
                               [ rdf:type owl:Class ;
                                 owl:complementOf sulo:Process
                               ] ;
                    rdfs:comment "has participant is a relation that describes the participation of a (non-process) thing in a process."@en ;
                    rdfs:label "has participant"@en .


###  https://w3id.org/sulo/isLocationOf
sulo:isLocationOf rdf:type owl:ObjectProperty ,
                           owl:TransitiveProperty ,
                           owl:ReflexiveProperty ;
                  rdfs:comment "A is location of B iff the spatialtemporal region occupied by A is the spatialtemporal region occupied by B."@en ;
                  rdfs:label "is location of"@en .


###  https://w3id.org/sulo/occursIn
sulo:occursIn rdf:type owl:ObjectProperty ;
              rdfs:subPropertyOf owl:topObjectProperty ;
              rdfs:domain owl:Thing ;
              rdfs:range sulo:Time ;
              rdfs:comment "a relation between any thing and the time in which it occurs in."@en ;
              rdfs:label "occurs in"@en .


###  https://w3id.org/sulo/precedes
sulo:precedes rdf:type owl:ObjectProperty ;
              rdfs:domain sulo:Process ;
              rdfs:range sulo:Process ;
              rdfs:comment "A relation in which one process occurs prior to another process."@en ;
              rdfs:label "precedes" .


###  https://w3id.org/sulo/refersTo
sulo:refersTo rdf:type owl:ObjectProperty ;
              rdfs:label "refers to"@en .


###  https://w3id.org/sulo/represents
sulo:represents rdf:type owl:ObjectProperty ;
                rdfs:subPropertyOf sulo:refersTo ;
                rdfs:comment "a represents b when a serves as a sign, symbol or model of b."@en ;
                rdfs:label "represents"@en .


#################################################################
#    Data properties
#################################################################

###  https://w3id.org/sulo/hasValue
sulo:hasValue rdf:type owl:DatatypeProperty ;
              rdfs:domain sulo:InformationObject ;
              rdfs:comment "has value is the (only) data type attribute to store the values of information objects."@en ;
              rdfs:label "has value"@en .


#################################################################
#    Classes
#################################################################

###  https://w3id.org/sulo/ActionSpecification
sulo:ActionSpecification rdf:type owl:Class ;
                         rdfs:subClassOf sulo:InformationObject ;
                         rdfs:comment "An action specification is an information object composed of a sequence of instructions to achieve some objective"@en ;
                         rdfs:label "action specification"@en .


###  https://w3id.org/sulo/Attribute
sulo:Attribute rdf:type owl:Class ;
               rdfs:subClassOf [ rdf:type owl:Restriction ;
                                 owl:onProperty [ owl:inverseOf sulo:hasAttribute
                                                ] ;
                                 owl:someValuesFrom [ rdf:type owl:Class ;
                                                      owl:unionOf ( sulo:Object
                                                                    sulo:Process
                                                                  )
                                                    ]
                               ] ;
               owl:disjointUnionOf ( sulo:Capability
                                     sulo:Quality
                                     sulo:Role
                                   ) ;
               rdfs:comment "An attribute is a property of an object or process that stems from their intrisinc structure and/or contextual interactions."@en ;
               rdfs:label "attribute"@en .


###  https://w3id.org/sulo/Capability
sulo:Capability rdf:type owl:Class ;
                rdfs:subClassOf sulo:Attribute ;
                rdfs:comment "A capability is an attribute that describes what an entity is able to do, under some set of circumstances."@en ,
                             "the capability to fly, the capabilty to reduce the activation energy of a chemical reaction, the capability to reason"@en ;
                rdfs:label "capability" .


###  https://w3id.org/sulo/Duration
sulo:Duration rdf:type owl:Class ;
              rdfs:subClassOf sulo:TimeInterval ;
              rdfs:label "duration"@en .


###  https://w3id.org/sulo/EndTime
sulo:EndTime rdf:type owl:Class ;
             rdfs:subClassOf sulo:TimeInstant ;
             rdfs:label "end time"@en .


###  https://w3id.org/sulo/InformationObject
sulo:InformationObject rdf:type owl:Class ;
                       rdfs:subClassOf sulo:Object ,
                                       [ rdf:type owl:Restriction ;
                                         owl:onProperty sulo:hasPart ;
                                         owl:allValuesFrom sulo:InformationObject
                                       ] ;
                       owl:disjointWith sulo:SpatialObject ;
                       rdfs:comment "an information object is an object that represents or encodes information. Information objects can be stored, transmitted, or processed to enable communication, reasoning, or decision-making."@en ;
                       rdfs:label "information object"@en .


###  https://w3id.org/sulo/Object
sulo:Object rdf:type owl:Class ;
            rdfs:subClassOf [ rdf:type owl:Class ;
                              owl:complementOf [ rdf:type owl:Restriction ;
                                                 owl:onProperty sulo:hasPart ;
                                                 owl:someValuesFrom sulo:Process
                                               ]
                            ] ,
                            [ rdf:type owl:Restriction ;
                              owl:onProperty sulo:hasPart ;
                              owl:allValuesFrom sulo:Object
                            ] ;
            owl:disjointWith sulo:Process ;
            rdfs:comment "An object is an entity that maintains its identity through time, and does not have temporal parts." ;
            rdfs:label "object"@en .


###  https://w3id.org/sulo/Process
sulo:Process rdf:type owl:Class ;
             rdfs:subClassOf [ rdf:type owl:Restriction ;
                               owl:onProperty sulo:hasPart ;
                               owl:allValuesFrom sulo:Process
                             ] ;
             rdfs:comment "a process is a entity that unfolds in time and has temporal parts."@en ;
             rdfs:label "process"@en .


###  https://w3id.org/sulo/Quality
sulo:Quality rdf:type owl:Class ;
             rdfs:subClassOf sulo:Attribute ;
             owl:disjointWith sulo:Role ;
             rdfs:comment "A quality is an attribute that is intrinsically associated with its bearer (or its parts)."@en ,
                          "the color of an apple, the smoothness of skin, the brightness of a star, the speed of an event"@en ;
             rdfs:label "quality"@en .


###  https://w3id.org/sulo/Quantity
sulo:Quantity rdf:type owl:Class ;
              rdfs:subClassOf sulo:InformationObject ;
              rdfs:comment "A quantity is an informational object that contains the magnitude (and unit) of an attribute."@en ;
              rdfs:label "quantity"@en .


###  https://w3id.org/sulo/Role
sulo:Role rdf:type owl:Class ;
          rdfs:subClassOf sulo:Attribute ;
          rdfs:comment "A role is an attribute that describes a context-dependent behaviour."@en ,
                       "a teacher, a student, a catalyst, a substrate, a product"@en ;
          rdfs:label "role"@en .


###  https://w3id.org/sulo/Set
sulo:Set rdf:type owl:Class ;
         rdfs:subClassOf sulo:InformationObject ;
         rdfs:comment "A set is a collection of things, for which there may be zero members."@en ;
         rdfs:label "set"@en .


###  https://w3id.org/sulo/SpatialObject
sulo:SpatialObject rdf:type owl:Class ;
                   rdfs:subClassOf sulo:Object ,
                                   [ rdf:type owl:Restriction ;
                                     owl:onProperty sulo:hasPart ;
                                     owl:allValuesFrom sulo:SpatialObject
                                   ] ;
                   rdfs:comment "A spatial object is an object that occupies space"@en ;
                   rdfs:label "spatial object"@en ;
                   <http://www.w3.org/2004/02/skos/core#example> "a mountain, a planet, a photon, the lining of the stomach, the cavity of the stomach, the space between mars and earth"@en .


###  https://w3id.org/sulo/StartTime
sulo:StartTime rdf:type owl:Class ;
               rdfs:subClassOf sulo:TimeInstant ;
               rdfs:label "start time"@en .


###  https://w3id.org/sulo/Time
sulo:Time rdf:type owl:Class ;
          rdfs:subClassOf sulo:Quantity ,
                          [ rdf:type owl:Restriction ;
                            owl:onProperty sulo:hasPart ;
                            owl:someValuesFrom sulo:Unit
                          ] ;
          rdfs:comment "time is a quantity pertaining to the duration of some interval of time or a particular instant of time (against some frame of reference)."@en ;
          rdfs:label "time"@en .


###  https://w3id.org/sulo/TimeInstant
sulo:TimeInstant rdf:type owl:Class ;
                 rdfs:subClassOf sulo:Time ;
                 rdfs:label "time instant"@en .


###  https://w3id.org/sulo/TimeInterval
sulo:TimeInterval rdf:type owl:Class ;
                  rdfs:subClassOf sulo:Time ;
                  rdfs:label "time interval" .


###  https://w3id.org/sulo/Unit
sulo:Unit rdf:type owl:Class ;
          rdfs:subClassOf sulo:Quantity ;
          rdfs:label "unit" .


###  Generated by the OWL API (version 4.5.26.2023-07-17T20:34:13Z) https://github.com/owlcs/owlapi
