@prefix dc: <http://purl.org/dc/elements/1.1/> .
@prefix dcat: <http://www.w3.org/ns/dcat#> .
@prefix dcterms: <http://purl.org/dc/terms/> .
@prefix foaf: <http://xmlns.com/foaf/0.1/> .
@prefix mod: <https://w3id.org/mod#> .
@prefix omv: <http://omv.ontoware.org/2005/05/ontology#> .
@prefix owl: <http://www.w3.org/2002/07/owl#> .
@prefix pav: <http://purl.org/pav/> .
@prefix rdf: <http://www.w3.org/1999/02/22-rdf-syntax-ns#> .
@prefix rdfs: <http://www.w3.org/2000/01/rdf-schema#> .
@prefix schema: <https://schema.org/> .
@prefix skos: <http://www.w3.org/2004/02/skos/core#> .
@prefix sulo: <https://w3id.org/sulo/> .
@prefix vann: <http://purl.org/vocab/vann/> .
@prefix xsd: <http://www.w3.org/2001/XMLSchema#> .

dc:creator a owl:AnnotationProperty .

dcterms:alternative a owl:AnnotationProperty .

dcterms:contributor a owl:AnnotationProperty .

dcterms:created a owl:AnnotationProperty .

dcterms:issued a owl:AnnotationProperty .

dcterms:language a owl:AnnotationProperty .

dcterms:license a owl:AnnotationProperty .

dcterms:modified a owl:AnnotationProperty .

dcterms:publisher a owl:AnnotationProperty .

dcterms:title a owl:AnnotationProperty .

pav:authoredBy a owl:AnnotationProperty .

vann:preferredNamespacePrefix a owl:AnnotationProperty .

vann:preferredNamespaceUri a owl:AnnotationProperty .

skos:example a owl:AnnotationProperty .

dcat:accessURL a owl:AnnotationProperty .

foaf:homepage a owl:AnnotationProperty .

schema:funding a owl:AnnotationProperty .

mod:definitionProperty a owl:AnnotationProperty .

mod:hasRepresentationLanguage a owl:AnnotationProperty .

mod:hasSyntax a owl:AnnotationProperty .

mod:prefLabelProperty a owl:AnnotationProperty .

sulo:atTime a owl:ObjectProperty ;
    rdfs:label "at time"@en ;
    dcterms:alternative "existsAt"@en ;
    rdfs:comment "a relation between any thing and the time in which it occurs at."@en ;
    rdfs:domain owl:Thing ;
    rdfs:range sulo:Time ;
    owl:inverseOf sulo:isTimeOf .

sulo:isPrecededBy a owl:ObjectProperty ;
    rdfs:label "is preceded by"@en ;
    rdfs:comment "A relation in which one process occurs after to another process."@en ;
    rdfs:domain sulo:Process ;
    rdfs:range sulo:Process ;
    owl:inverseOf sulo:precedes .

sulo:isReferredIn a owl:ObjectProperty ;
    rdfs:label "is referred in"@en ;
    rdfs:comment "is referred in is relation between an object that is the subject of an information object."@en ;
    rdfs:domain owl:Thing ;
    rdfs:range sulo:InformationObject ;
    owl:inverseOf sulo:refersTo .

xsd:date a rdfs:Datatype .

sulo:EndTime a owl:Class ;
    rdfs:label "end time"@en ;
    rdfs:comment "an end time is a time instant at the end of a process/time interval."@en ;
    rdfs:subClassOf sulo:TimeInstant ;
    owl:disjointWith sulo:StartTime .

sulo:hasFeature a owl:ObjectProperty ;
    rdfs:label "has feature"@en ;
    rdfs:comment "has feature is a relation between a thing and an internal, contextual, or externally attributed characteristic."@en ;
    rdfs:domain [ a owl:Class ;
            owl:unionOf ( sulo:Object sulo:Process ) ] ;
    rdfs:range sulo:Feature ;
    owl:inverseOf sulo:isFeatureOf .

sulo:hasMember a owl:ObjectProperty ;
    rdfs:label "has item"@en ;
    rdfs:comment "has item is a relation between a collection and an item contained therein."@en ;
    rdfs:domain sulo:Collection ;
    rdfs:range owl:Thing ;
    owl:inverseOf sulo:isItemIn .

sulo:hasParticipant a owl:ObjectProperty ;
    rdfs:label "has participant"@en ;
    rdfs:comment "has participant is a relation that describes the participation of a (non-process) thing in a process."@en ;
    rdfs:domain sulo:Process ;
    rdfs:range sulo:Object ;
    owl:inverseOf sulo:isParticipantIn ;
    owl:propertyChainAxiom ( sulo:hasParticipant [ owl:inverseOf sulo:hasFeature ] ) .

sulo:isDirectPartOf a owl:ObjectProperty ;
    rdfs:label "is direct part of"@en ;
    rdfs:comment "is direct part is a non-transitive parthood relation that can be used to specify cardinality constraints between a part and its whole."@en ;
    rdfs:subPropertyOf sulo:isPartOf .

sulo:isItemIn a owl:ObjectProperty ;
    rdfs:label "is item in"@en ;
    rdfs:comment "has item is a relation between an item and the collection in which it contained."@en ;
    rdfs:domain owl:Thing ;
    rdfs:range sulo:Collection ;
    rdfs:subPropertyOf owl:topObjectProperty .

sulo:isLocatedIn a owl:ObjectProperty,
        owl:TransitiveProperty ;
    rdfs:label "is in"@en ;
    rdfs:comment "A binary relation where the object entity includes the subject entity within its spatial, temporal, structural, or conceptual extent."@en ;
    rdfs:subPropertyOf owl:topObjectProperty ;
    owl:inverseOf sulo:isLocationOf .

sulo:isParticipantIn a owl:ObjectProperty ;
    rdfs:label "is participant in"@en ;
    rdfs:comment "is participant in is a relation to relate an object and the process in which it participates."@en ;
    rdfs:domain sulo:Object ;
    rdfs:range sulo:Process .

sulo:isTimeOf a owl:ObjectProperty ;
    rdfs:label "is time of" ;
    rdfs:comment "a relation between a time and an object that occurs within it."@en ;
    rdfs:domain sulo:Time ;
    rdfs:range owl:Thing .

sulo:precedes a owl:ObjectProperty ;
    rdfs:label "precedes" ;
    rdfs:comment "A relation in which one process occurs prior to another process."@en ;
    rdfs:domain sulo:Process ;
    rdfs:range sulo:Process .

sulo:refersTo a owl:ObjectProperty ;
    rdfs:label "refers to"@en ;
    rdfs:comment "refers to is a binary relation between an information object and any other object that it mentions, describes, represents, encodes, or otherwise provides information about."@en ;
    rdfs:domain sulo:InformationObject ;
    rdfs:range owl:Thing .

sulo:sulo-0.2.1.ttl a owl:Ontology ;
    rdfs:label "Simplified Upper Level Ontology"@en ;
    dc:creator <https://orcid.org/0000-0003-4727-9435> ;
    dcterms:alternative "SULO"@en ;
    dcterms:contributor <https://orcid.org/0000-0001-7222-3287> ;
    dcterms:created "2024-11-11" ;
    dcterms:issued "2025-07-11" ;
    dcterms:language <http://lexvo.org/id/iso639-1/en> ;
    dcterms:license <https://creativecommons.org/publicdomain/zero/1.0> ;
    dcterms:modified "2025-07-31"^^xsd:date ;
    dcterms:publisher <https://orcid.org/0000-0003-4727-9435> ;
    dcterms:title "Simplified Upper Level Ontology"@en ;
    pav:authoredBy <https://orcid.org/0000-0003-4727-9435> ;
    vann:preferredNamespacePrefix "sulo" ;
    vann:preferredNamespaceUri sulo: ;
    rdfs:comment "The Simplified Upper Level Ontology (SULO) is ontology with a minimal set of classes and relations to guide the development of a personal health knowledge graph."@en ;
    owl:versionIRI sulo:sulo-0.2.1.ttl ;
    owl:versionInfo "0.2.1" ;
    dcat:accessURL sulo:sulo.ttl ;
    foaf:homepage <https://github.com/AIDAVA-DEV/sulo> ;
    schema:funding "This work is partially supported by the AIDAVA project (GA 101057062), as part of the European Union's Horizon Europe research and innovation programme."@en ;
    mod:definitionProperty rdfs:comment ;
    mod:hasRepresentationLanguage omv:OWL ;
    mod:hasSyntax <http://www.w3.org/ns/formats/Turtle> ;
    mod:prefLabelProperty rdfs:label .

sulo:Capability a owl:Class ;
    rdfs:label "capability" ;
    rdfs:comment "A capability is a feature that describes what an entity is able to do, under some set of circumstances."@en ;
    rdfs:subClassOf sulo:Feature ;
    skos:example "the capability to fly, the capabilty to reduce the activation energy of a chemical reaction, the capability to reason"@en .

sulo:Collection a owl:Class ;
    rdfs:label "collection"@en ;
    rdfs:comment "A collection is an information object for which there may be zero or more items."@en ;
    rdfs:subClassOf [ a owl:Restriction ;
            owl:allValuesFrom owl:Thing ;
            owl:onProperty sulo:hasMember ],
        sulo:InformationObject ;
    owl:disjointWith sulo:Quantity ;
    skos:example "a stamp collection, a murder of crows, the arm of a clinical trial"@en .

sulo:Quality a owl:Class ;
    rdfs:label "quality"@en ;
    rdfs:comment "A quality is a feature that is intrinsically associated with its bearer (or its parts)."@en,
        "the color of an apple, the smoothness of skin, the brightness of a star, the speed of an event"@en ;
    rdfs:subClassOf sulo:Feature .

sulo:Role a owl:Class ;
    rdfs:label "role"@en ;
    rdfs:comment "A role is a feature that describes a context-dependent behaviour."@en ;
    rdfs:subClassOf sulo:Feature ;
    skos:example "a teacher, a student, a catalyst, a substrate, a product, a patient"@en .

sulo:SpatialObject a owl:Class ;
    rdfs:label "spatial object"@en ;
    rdfs:comment "A spatial object is an object that occupies space"@en ;
    rdfs:subClassOf [ a owl:Restriction ;
            owl:allValuesFrom sulo:SpatialObject ;
            owl:onProperty sulo:hasPart ],
        sulo:Object ;
    skos:example "a mountain, a planet, a photon, the lining of the stomach, the cavity of the stomach, the space between mars and earth"@en .

sulo:StartTime a owl:Class ;
    rdfs:label "start time"@en ;
    rdfs:comment "a start time is a time instant at the beginning of a process/time interval."@en ;
    rdfs:subClassOf sulo:TimeInstant .

sulo:TimeInterval a owl:Class ;
    rdfs:label "time interval" ;
    rdfs:comment "A time interval is a quantity for a continuous and bounded extent of time, characterized by a start time and an end time."@en ;
    rdfs:subClassOf [ a owl:Restriction ;
            owl:onProperty sulo:hasDirectPart ;
            owl:someValuesFrom sulo:EndTime ],
        [ a owl:Restriction ;
            owl:onProperty sulo:hasDirectPart ;
            owl:someValuesFrom sulo:StartTime ],
        [ a owl:Restriction ;
            owl:onProperty sulo:hasPart ;
            owl:someValuesFrom sulo:Duration ],
        [ a owl:Restriction ;
            owl:onProperty sulo:hasPart ;
            owl:someValuesFrom sulo:Unit ],
        [ a owl:Restriction ;
            owl:allValuesFrom xsd:float ;
            owl:onProperty sulo:hasValue ],
        sulo:Time .

sulo:hasDirectPart a owl:ObjectProperty ;
    rdfs:label "has direct part" ;
    rdfs:comment "has direct part is a non-transitive parthood relation that can be used to specify cardinality constraints between a whole and its parts."@en ;
    rdfs:subPropertyOf sulo:hasPart ;
    owl:inverseOf sulo:isDirectPartOf .

sulo:isFeatureOf a owl:ObjectProperty ;
    rdfs:label "is feature of"@en ;
    rdfs:comment "is feature of is a relation between an internal, contextual, or externally attributed characteristic and some Thing."@en ;
    rdfs:domain sulo:Feature ;
    rdfs:range [ a owl:Class ;
            owl:unionOf ( sulo:Object sulo:Process ) ] .

sulo:isLocationOf a owl:ObjectProperty,
        owl:TransitiveProperty ;
    rdfs:label "contains"@en ;
    rdfs:comment "A binary relation where the subject entity includes the object entity within its spatial, temporal, structural, or conceptual extent."@en .

sulo:isPartOf a owl:ObjectProperty,
        owl:ReflexiveProperty,
        owl:TransitiveProperty ;
    rdfs:label "is part of"@en ;
    rdfs:comment "is part of is a transitive, reflexive and antisymmetric relation between a part and itself or a part and a whole."@en ;
    rdfs:subPropertyOf sulo:isLocatedIn .

sulo:Duration a owl:Class ;
    rdfs:label "duration"@en ;
    rdfs:comment "Duration is a temporal quantity that represents the extent or (non-negative) amount of time that elapses between two temporal points, typically the start and end of a time interval."@en ;
    rdfs:subClassOf [ a owl:Restriction ;
            owl:onProperty sulo:hasValue ;
            owl:someValuesFrom [ a rdfs:Datatype ;
                    owl:onDatatype xsd:float ;
                    owl:withRestrictions ( [ xsd:minInclusive "0.0"^^xsd:float ] ) ] ],
        sulo:Time .

sulo:Quantity a owl:Class ;
    rdfs:label "quantity"@en ;
    rdfs:comment "A quantity is an informational object that contains the magnitude (and unit) of an attribute."@en ;
    rdfs:subClassOf [ a owl:Restriction ;
            owl:onProperty sulo:hasPart ;
            owl:someValuesFrom sulo:Unit ],
        sulo:InformationObject .

sulo:Unit a owl:Class ;
    rdfs:label "unit" ;
    rdfs:comment "a unit is a standardized quantity that is used as a reference for a particular quantity."@en ;
    rdfs:subClassOf sulo:Quantity .

sulo:TimeInstant a owl:Class ;
    rdfs:label "time instant"@en ;
    rdfs:comment "time instant is a quantity of time a particular moment in time."@en ;
    rdfs:subClassOf [ a owl:Restriction ;
            owl:allValuesFrom [ a rdfs:Datatype ;
                    owl:unionOf ( xsd:date xsd:dateTime xsd:dateTimeStamp ) ] ;
            owl:onProperty sulo:hasValue ],
        sulo:Time .

sulo:hasValue a owl:DatatypeProperty,
        owl:FunctionalProperty ;
    rdfs:label "has value"@en ;
    rdfs:comment "has value is the (only) data type attribute to store the values of information objects."@en ;
    rdfs:domain sulo:InformationObject .

sulo:Time a owl:Class ;
    rdfs:label "time"@en ;
    rdfs:comment "time is a quantity pertaining to the duration of some interval of time or a particular instant of time (against some frame of reference)."@en ;
    rdfs:subClassOf sulo:Quantity ;
    owl:disjointUnionOf ( sulo:Duration sulo:TimeInstant sulo:TimeInterval ) ;
    owl:disjointWith sulo:Unit .

sulo:Feature a owl:Class ;
    rdfs:label "feature"@en ;
    rdfs:comment "A feature is any characteristic that stems from the intrisinc structure and/or context"@en ;
    rdfs:subClassOf [ a owl:Restriction ;
            owl:onProperty sulo:isFeatureOf ;
            owl:someValuesFrom [ a owl:Class ;
                    owl:unionOf ( sulo:Object sulo:Process ) ] ],
        [ a owl:Restriction ;
            owl:allValuesFrom sulo:Feature ;
            owl:onProperty sulo:hasPart ],
        sulo:Object ;
    owl:disjointUnionOf ( sulo:Capability sulo:InformationObject sulo:Quality sulo:Role ) ;
    owl:disjointWith sulo:SpatialObject ;
    skos:example "the capability to fly, a collection of cards, a measured height of 170cm."@en .

sulo:InformationObject a owl:Class ;
    rdfs:label "information object"@en ;
    rdfs:comment "an information object is a feature that represents, is about, or encodes some information."@en ;
    rdfs:subClassOf [ a owl:Restriction ;
            owl:allValuesFrom sulo:InformationObject ;
            owl:onProperty sulo:hasPart ],
        [ a owl:Restriction ;
            owl:allValuesFrom rdfs:Literal ;
            owl:onProperty sulo:hasValue ],
        sulo:Feature .

sulo:Object a owl:Class ;
    rdfs:label "object"@en ;
    rdfs:comment "An object is an entity that maintains its identity through time, and does not have processes as its parts." ;
    rdfs:subClassOf [ a owl:Class ;
            owl:complementOf [ a owl:Restriction ;
                    owl:onProperty sulo:hasPart ;
                    owl:someValuesFrom sulo:Process ] ],
        [ a owl:Restriction ;
            owl:allValuesFrom sulo:Object ;
            owl:onProperty sulo:hasPart ] ;
    owl:disjointWith sulo:Process ;
    skos:example "a heart, the function to pump blood, the role of a doctor"@en .

sulo:hasPart a owl:ObjectProperty,
        owl:ReflexiveProperty,
        owl:TransitiveProperty ;
    rdfs:label "has part"@en ;
    rdfs:comment "has part is a transitive, reflexive and antisymmetric relation between a whole and itself or a whole and its part." ;
    rdfs:subPropertyOf sulo:isLocationOf ;
    owl:inverseOf sulo:isPartOf .

sulo:Process a owl:Class ;
    rdfs:label "process"@en ;
    rdfs:comment "a process is a entity that unfolds in time, has temporal parts, and has objects that participate in the process."@en ;
    rdfs:subClassOf [ a owl:Restriction ;
            owl:allValuesFrom sulo:Process ;
            owl:onProperty sulo:hasPart ] ;
    skos:example "the process of diagnosing a problem condition, the process of walking down the street, the process of teaching a class"@en .

[] a owl:AllDisjointClasses ;
    owl:members ( sulo:Capability sulo:InformationObject sulo:Quality sulo:Role ) .

[] a owl:AllDisjointClasses ;
    owl:members ( sulo:Duration sulo:TimeInstant sulo:TimeInterval ) .

